More work on the VDM model, mechanised Dwarf up to the operations and added a script to generate HTML from a LaTeX file of laws.

gen_laws.py
@@ -1,0 +1,16 @@
+#!/usr/bin/python
+
+import sys
+import re
+
+if len(sys.argv) < 2:
+  print "Please supply a filename to process"
+  sys.exit()
+
+content = open(sys.argv[1], "r").read()
+
+finds = re.findall('\\\\isacommand{theorem}.*%\n[^%]*',content)
+
+print('\n<p>There are currently ' + str(len(finds)) + ' laws in this theory</p>\n')
+
+print('\n\n'.join(map(lambda x: "<p>\n$" + x + "$\n</p>", finds)))
