theories/models/utp_vdm_simple/examples/Dwarf.thy
@@ -1,27 +1,121 @@
 theory Dwarf
 imports 
-  "../utp_vdm_types"
-  "../utp_vdm_functions"
+  "../utp_vdm"
 begin
 
 abbreviation "L1 \<equiv> ''L1''"
 abbreviation "L2 \<equiv> ''L2''"
 abbreviation "L3 \<equiv> ''L3''"
 
-abbreviation "LampId   \<equiv> &<L1> | <L2> | <L3>&"
-abbreviation "Signal   \<equiv> &@set of @LampId&"
-abbreviation "dark     \<equiv> *{}*"
-abbreviation "stop     \<equiv> *{<L1>, <L2>}*"
-abbreviation "warning  \<equiv> *{<L1>, <L3>}*"
-abbreviation "drive    \<equiv> *{<L2>, <L3>}*"
+text {* First set of VDM types, which depend on nothing else *}
 
-syntax
-  "_vexpr_vexpr"  :: "'a vdme \<Rightarrow> vexpr" ("@_")
+abbreviation "LampId   \<equiv> \<parallel><L1> | <L2> | <L3>\<parallel>"
+abbreviation "Signal   \<equiv> \<parallel>@set of @LampId\<parallel>"
 
-translations
-  "_vexpr_vexpr x" => "x"
+text {* Next define the "proper states" for the signal *}
 
-abbreviation "ProperState \<equiv> &@Signal inv ps == (!ps! in set {@dark, @stop, @warning, @drive})&"
+definition "dark     \<equiv> |{}|"
+definition "stop     \<equiv> |{<L1>, <L2>}|"
+definition "warning  \<equiv> |{<L1>, <L3>}|"
+definition "drive    \<equiv> |{<L2>, <L3>}|"
 
+text {* A proper state is a signal which falls within this set *}
+
+abbreviation 
+  "ProperState \<equiv> \<parallel>@Signal inv ps == (^ps^ in @set {@dark, @stop, @warning, @drive})\<parallel>"
+
+text {* Setting up a record type is currently a little complicated, though could
+        easily be automatically generated. First we create a new unit type to act
+        as the "tag" for this record so that it can be distinguished from others. We
+        create an instance of the tag class which proves its a unit type and associates
+        a string with it (the name of the type). *}
+
+typedef DwarfType_Tag = "{True}" by auto
+instantiation DwarfType_Tag :: tag
+begin
+definition "tagName_DwarfType_Tag (x::DwarfType_Tag) = ''DwarfType''"
+instance 
+  by (intro_classes, metis (full_types) Abs_DwarfType_Tag_cases singleton_iff)
+end
+
+text {* Next we create a collection of fields associated with the tag, and give each
+        the position in record and its VDM type. *}
+
+abbreviation "lastproperstate_fld    \<equiv> MkField TYPE(DwarfType_Tag) #1 \<parallel>@ProperState\<parallel>"
+abbreviation "desiredproperstate_fld \<equiv> MkField TYPE(DwarfType_Tag) #2 \<parallel>@ProperState\<parallel>"
+abbreviation "turnoff_fld            \<equiv> MkField TYPE(DwarfType_Tag) #3 \<parallel>@set of @LampId\<parallel>"
+abbreviation "turnon_fld             \<equiv> MkField TYPE(DwarfType_Tag) #4 \<parallel>@set of @LampId\<parallel>"
+abbreviation "laststate_fld          \<equiv> MkField TYPE(DwarfType_Tag) #5 \<parallel>@Signal\<parallel>"
+abbreviation "currentstate_fld       \<equiv> MkField TYPE(DwarfType_Tag) #6 \<parallel>@Signal\<parallel>"
+
+text {* Then we use these fields to create selector functions for the record, which
+        can be used directly in UTP/VDM predicates *}
+
+abbreviation "lastproperstate    \<equiv> SelectRec lastproperstate_fld"
+abbreviation "desiredproperstate \<equiv> SelectRec desiredproperstate_fld"
+abbreviation "turnoff            \<equiv> SelectRec turnoff_fld"
+abbreviation "turnon             \<equiv> SelectRec turnon_fld"
+abbreviation "laststate          \<equiv> SelectRec laststate_fld"
+abbreviation "currentstate       \<equiv> SelectRec currentstate_fld"
+
+text {* Finally we create the actual type by giving the list of fields and the associated
+        invariant. We also create a record constructor, mk_DwarfType. *}
+
+abbreviation 
+  "DwarfType \<equiv> \<parallel>[ lastproperstate_fld
+                , desiredproperstate_fld
+                , turnoff_fld
+                , turnon_fld
+                , laststate_fld
+                , currentstate_fld] 
+                inv d == ((^d^.currentstate setminus ^d^.turnoff) union ^d^.turnon 
+                            = ^d^.desiredproperstate)
+                         and 
+                         (^d^.turnon inter ^d^.turnoff = {})\<parallel>"
+
+definition "mk_DwarfType \<equiv> MkRec DwarfType"
+
+text {* The Dwarf Signal has a single state variable which gives 
+        the state of the signal. *}
+
+definition "dw \<equiv> MkVarD ''dw'' DwarfType"
+
+text {* Next we create the different operations for the Dwarf signal 
+        as UTP designs. Probably these should be reactive designs. *}
+
+definition "Init = `true \<turnstile> dw := mk_DwarfType(@stop, {}, {}, @stop, @stop, @stop)`"
+
+lemma "`Init ; Init` = `Init`"
+  apply (unfold Init_def)
+
+definition 
+  "SetNewProperState st = 
+      `\<lparr>($dw).currentstate = ($dw).desiredproperstate and ^st^ <> ($dw).currentstate\<rparr> 
+       \<turnstile> dw := mk_DwarfType( ($dw).currentstate
+                           , ($dw).currentstate setminus ^st^
+                           , ^st^ setminus ($dw).currentstate
+                           , ($dw).laststate
+                           , ($dw).currentstate
+                           , ^st^)`"
+
+definition
+  "TurnOn l =
+     `\<lparr> ^l^ in @set ($dw).turnon \<rparr> 
+      \<turnstile> dw := mk_DwarfType( ($dw).lastproperstate
+                          , ($dw).turnoff setminus {^l^}
+                          , ($dw).turnon setminus {^l^}
+                          , ($dw).currentstate
+                          , ($dw).currentstate union {^l^}
+                          , ($dw).desiredproperstate)`"
+
+definition
+  "TurnOff l =
+     `\<lparr> ^l^ in @set ($dw).turnoff \<rparr> 
+      \<turnstile> dw := mk_DwarfType( ($dw).lastproperstate
+                          , ($dw).turnoff setminus {^l^}
+                          , ($dw).turnon setminus {^l^}
+                          , ($dw).currentstate
+                          , ($dw).currentstate setminus {^l^}
+                          , ($dw).desiredproperstate)`"
 
 end
